finish prelim lrat soundness

examples/lrat_checker/lratScript.sml
@@ -1,73 +1,9 @@
 (*
-   Verification of longest common subsequence algorithms.
+   Verification of LRAT checker
 *)
 open preamble miscTheory;
 
 val _ = new_theory "lrat";
-
-(*** Implementation ***
-
-  The concrete notion of a literal is an integer
-  To reduce symmetries the literal "0" is just lumped in as well although it doesn't have a -0
-
-  A clause is a list of literals and a formula is a set of clauses
-
-*)
-val _ = type_abbrev("clause" , ``:int list``);
-
-(* NOTE: not efficient! *)
-val delete_literal_def = Define`
-  delete_literal l (C:clause) =
-    FILTER (λi. i  <> l) C `
-
-val _ = Datatype`
-  lratstep =
-    Delete (num list) (* Clauses to delete *)
-  | RAT num clause (num list)`
-    (* TODO: For now, an Asymmetric Tautology step
-      AT n C i0
-      i0 is a list of clause IDs
-      n is the new id of the clause C
-    *)
-
-val _ = type_abbrev("lrat" , ``:lratstep list``);
-
-val delete_clauses_def = Define`
-  delete_clauses cl fml =
-    FOLDR delete fml cl`
-
-(* asymmetric tautology step *)
-val is_AT_def = Define`
-  (is_AT fml [] (C:clause) = F) ∧
-  (is_AT fml (i::is) C =
-  case lookup i fml of
-    NONE => F
-  | SOME Ci =>
-  let D = FILTER (λx. ¬ MEM x C) Ci
-  in
-  case D of
-    [] => T
-  | [d] => is_AT fml is (-d::C)
-  | _ => F)`
-
-val wf_clause_def = Define`
-  wf_clause (C:clause) ⇔ ¬MEM 0 C`
-
-(* Run the LRAT checker on fml, returning an  *)
-val check_lrat_def = Define`
-  (check_lrat [] fml = SOME fml) ∧
-  (check_lrat (step::steps) fml =
-    case step of
-      Delete cl =>
-      check_lrat steps (delete_clauses cl fml)
-    | RAT n C cl =>
-      if wf_clause C ∧ is_AT fml cl C
-      (* Are overwrites allowed???
-      if n ∈ domain fml then NONE
-      else *)
-      (* TODO: insert check that it is indeed okay *)
-      then check_lrat steps (insert n C fml)
-      else NONE)`
 
 (*** Semantics ***
 
@@ -75,14 +11,15 @@ val check_lrat_def = Define`
   It would be worth defining a more abstract notion of this that doesn't mess
   concretely with -1,1 etc.
 
+  A clause is a list of literals (ints)
+  A CNF is a set of clauses
+
   An assignment is a map from the natural numbers (including 0) to T/F
 
-  A clause is satisfied if there is at least one literal assigned to true
-
-  A CNF is satisfied if there is at all clauses are satisfied
-
+  A clause is satisfied by an assignment if there is at least one of its literals assigned to true
+  A CNF is satisfied by an assignment if all its clauses are satisfied
 *)
-
+val _ = type_abbrev("clause" , ``:int list``);
 val _ = type_abbrev("cnf" , ``:clause set``);
 val _ = type_abbrev("assignment" , ``:num -> bool``);
 
@@ -105,7 +42,9 @@ val satisfiable_def = Define`
 val unsatisfiable_def = Define`
   unsatisfiable fml ⇔ ¬satisfiable fml`
 
-(*** Proofs about abstract notion ***)
+(*** Proofs about the semantics ***)
+
+(* General stuff about satisfiability *)
 
 (* Empty clauses are unsat *)
 Theorem empty_clause_imp_unsatisfiable:
@@ -116,7 +55,7 @@ Proof
   qexists_tac`[]`>> simp[]
 QED
 
-(* Deleting any set of clauses preserves satisfiability *)
+(* l , -l are duals *)
 Theorem satisfies_literal_exclusive:
   l ≠ 0 ⇒
   (satisfies_literal w l ⇔  ¬satisfies_literal w (-l))
@@ -124,12 +63,6 @@ Proof
   rw[EQ_IMP_THM,satisfies_literal_def]>>
   fs[] >> `F` by intLib.ARITH_TAC
 QED
-
-(* Asymmetric tautologies *)
-val asymmetric_tautology_def = Define`
-  asymmetric_tautology fml C ⇔
-  ¬MEM 0 C ∧
-  unsatisfiable (fml ∪ set (MAP (λl. [-l]) C))`
 
 Theorem unsat_negate_satisfies_literal:
   l ≠ 0 ∧ unsatisfiable ([-l] INSERT fml) ∧
@@ -146,13 +79,6 @@ Proof
     metis_tac[]
 QED
 
-Theorem satisfies_union:
-  satisfies w (A ∪ B) ⇔ satisfies w A ∧ satisfies w B
-Proof
-  rw[satisfies_def]>>
-  metis_tac[]
-QED
-
 Theorem satisfies_INSERT:
   satisfies w (C INSERT fml) ⇔ satisfies_clause w C ∧ satisfies w fml
 Proof
@@ -160,13 +86,73 @@ Proof
   metis_tac[]
 QED
 
+Theorem satisfies_SUBSET:
+  fml' ⊆ fml ⇒
+  satisfies w fml ⇒ satisfies w fml'
+Proof
+  rw[satisfies_def]>>
+  metis_tac[SUBSET_DEF]
+QED
+
 Theorem satisfiable_SUBSET:
   fml' ⊆ fml ⇒
   satisfiable fml ⇒ satisfiable fml'
 Proof
-  fs[satisfiable_def,satisfies_def]>>
-  metis_tac[SUBSET_DEF]
+  fs[satisfiable_def]>>
+  metis_tac[satisfies_SUBSET]
 QED
+
+Theorem satisfies_union:
+  satisfies w (A ∪ B) ⇔ satisfies w A ∧ satisfies w B
+Proof
+  rw[satisfies_def]>>
+  metis_tac[]
+QED
+
+Theorem satisfiable_DIFF:
+  satisfiable fml ⇒
+  satisfiable (fml DIFF clauses)
+Proof
+  fs[satisfiable_def,satisfies_def]>>
+  metis_tac[]
+QED
+
+Theorem sing_satisfies_literal:
+  [l] ∈ fml ∧
+  satisfies w fml ⇒
+  satisfies_literal w l
+Proof
+  rw[satisfies_def]>>
+  first_x_assum drule>>
+  fs[satisfies_clause_def]
+QED
+
+Theorem satisfies_clause_append:
+  satisfies_clause w (A++B) ⇔ satisfies_clause w A ∨ satisfies_clause w B
+Proof
+  fs[satisfies_clause_def]>>
+  metis_tac[]
+QED
+
+Theorem satisfies_clause_SUBSET:
+  (∀l. MEM l (C:clause) ⇒ MEM l C') ⇒
+  satisfies_clause w C ⇒ satisfies_clause w C'
+Proof
+  rw[satisfies_clause_def]>>
+  metis_tac[]
+QED
+
+Theorem UNION_INSERT_EQ:
+  A ∪ (B INSERT C) = B INSERT (A ∪ C)
+Proof
+  fs[EXTENSION]>>metis_tac[]
+QED
+
+(* Definition of asymmetric tautologies *)
+val asymmetric_tautology_def = Define`
+  asymmetric_tautology fml C ⇔
+  ¬MEM 0 C ∧
+  unsatisfiable (fml ∪ set (MAP (λl. [-l]) C))`
 
 Theorem list_unsat_negate_satisfies_literal:
   ∀ls.
@@ -181,25 +167,47 @@ Proof
   metis_tac[satisfies_literal_exclusive]
 QED
 
+Theorem asymmetric_tautology_satisfies:
+  ∀C fml.
+  asymmetric_tautology fml C ⇒
+  satisfies w fml ⇒
+  satisfies w (C INSERT fml)
+Proof
+  rw[asymmetric_tautology_def]>>
+  drule list_unsat_negate_satisfies_literal>>
+  disch_then drule>>
+  metis_tac[satisfies_INSERT]
+QED
+
 Theorem asymmetric_tautology_satisfiable:
   ∀C fml.
   asymmetric_tautology fml C ⇒
   satisfiable fml ⇒
   satisfiable (C INSERT fml)
 Proof
-  rw[satisfiable_def,asymmetric_tautology_def]>>
-  drule list_unsat_negate_satisfies_literal>>
-  disch_then drule>>
-  metis_tac[satisfies_INSERT]
+  rw[satisfiable_def]>>
+  metis_tac[asymmetric_tautology_satisfies]
 QED
 
-Theorem satisfiable_DIFF:
-  satisfiable fml ⇒
-  satisfiable (fml DIFF clauses)
+Theorem asymmetric_tautology_set_satisfies:
+  ∀Cs fml.
+  (∀C. C ∈ Cs ⇒ asymmetric_tautology fml C) ⇒
+  satisfies w fml ⇒
+  satisfies w (Cs ∪ fml)
 Proof
-  fs[satisfiable_def,satisfies_def]>>
-  metis_tac[]
+  rw[satisfies_union]>>
+  rw[satisfies_def]>>
+  first_x_assum drule>>
+  strip_tac>>
+  drule asymmetric_tautology_satisfies>>
+  disch_then drule>>
+  simp[satisfies_INSERT]
 QED
+
+(* TODO: NOT efficient *)
+val delete_literal_def = Define`
+  delete_literal l (C:clause) =
+    FILTER (λi. i  <> l) C `
 
 Theorem delete_literal_preserves_satisfies_clause:
   l ≠ 0 ∧ satisfies_literal w l ⇒
@@ -213,16 +221,6 @@ Proof
   >>
     fs[delete_literal_def,satisfies_clause_def,MEM_FILTER]>>
     metis_tac[]
-QED
-
-Theorem sing_satisfies_literal:
-  [l] ∈ fml ∧
-  satisfies w fml ⇒
-  satisfies_literal w l
-Proof
-  rw[satisfies_def]>>
-  first_x_assum drule>>
-  fs[satisfies_clause_def]
 QED
 
 Theorem delete_unit_preserves_satisfies:
@@ -241,8 +239,153 @@ Proof
   metis_tac[delete_unit_preserves_satisfies]
 QED
 
+(* Definition of resolution asymmetric tautology *)
+val resolution_asymmetric_tautology_def = Define`
+  resolution_asymmetric_tautology fml C ⇔
+  ¬MEM 0 C ∧
+  (asymmetric_tautology fml C ∨
+  ∃l. MEM l C ∧
+  ∀D. D ∈ fml ∧ MEM (-l) D ⇒
+    asymmetric_tautology fml (C ++ delete_literal (-l) D))`
+
+(* soundness of resolution step *)
+Theorem resolution_sound:
+  l ≠ 0 ∧ (l::xs) ∈ fml ∧ ((-l)::ys) ∈ fml ⇒
+  (satisfies w fml ⇔ satisfies w ((xs++ys) INSERT fml))
+Proof
+  simp[EQ_IMP_THM]>>strip_tac>>strip_tac
+  >- (
+    rw[satisfies_INSERT]>>
+    fs[satisfies_def]>>
+    first_assum drule>>
+    first_x_assum(qspec_then `l::xs` mp_tac)>>fs[]>>
+    rw[satisfies_clause_def,MEM_FILTER]>>
+    metis_tac[satisfies_literal_exclusive])
+  >>
+    match_mp_tac satisfies_SUBSET>>
+    fs[SUBSET_DEF]
+QED
+
+Theorem resolution_sound1:
+  l ≠ 0 ∧ xs ∈ fml ∧ ys ∈ fml ∧
+  MEM l xs ∧ MEM (-l) ys ⇒
+  (satisfies w fml ⇔ satisfies w ((xs++delete_literal (-l) ys) INSERT fml))
+Proof
+  simp[EQ_IMP_THM]>>strip_tac>>strip_tac
+  >- (
+    rw[satisfies_INSERT]>>
+    fs[satisfies_def]>>
+    first_assum drule>>
+    first_x_assum(qspec_then `xs` mp_tac)>>fs[]>>
+    rw[satisfies_clause_def]>>
+    metis_tac[satisfies_literal_exclusive])
+  >>
+    match_mp_tac satisfies_SUBSET>>
+    fs[SUBSET_DEF]
+QED
+
+val flip_literal_def = Define`
+  flip_literal l (w:assignment) =
+  λv. if v = Num (ABS l) then ¬w (Num (ABS l)) else w v`
+
+Theorem flip_literal_eq_neg:
+  flip_literal l w = flip_literal (-l) w
+Proof
+  simp[flip_literal_def]
+QED
+
+Theorem flip_literal_flips:
+  l ≠ 0 ⇒
+  (satisfies_literal w l ⇔ ¬(satisfies_literal (flip_literal l w) l))
+Proof
+  rw[satisfies_literal_def,flip_literal_def]
+QED
+
+Theorem flip_literal_unaffected:
+  l ≠ 0 ∧
+  satisfies_literal w l ∧
+  satisfies_clause w C ∧ ¬ MEM l C ⇒
+  satisfies_clause (flip_literal l w ) C
+Proof
+  rw[satisfies_clause_def,satisfies_literal_def]>>
+  asm_exists_tac>>fs[]>>rw[]>>fs[]>>
+  fs[flip_literal_def]>>
+  `l ≠ l'` by metis_tac[]>>
+  intLib.ARITH_TAC
+QED
+
+Theorem resolution_asymmetric_tautology_satisfiable:
+  ∀C fml w.
+  resolution_asymmetric_tautology fml C ⇒
+  satisfiable fml ⇒
+  satisfiable (C INSERT fml)
+Proof
+  rw[resolution_asymmetric_tautology_def]
+  >-
+    metis_tac[asymmetric_tautology_satisfiable]
+  >>
+  fs[satisfiable_def]>>
+  Cases_on`satisfies_clause w C`
+  >-
+    metis_tac[satisfies_INSERT]>>
+  qabbrev_tac`Ds = IMAGE (λD. C ++ delete_literal (-l) D) { D | D ∈ fml∧  MEM (-l) D}`>>
+  `∀D. D ∈ Ds ⇒ asymmetric_tautology fml D` by
+    (rw[]>>fs[Abbr`Ds`])>>
+  drule asymmetric_tautology_set_satisfies >>
+  disch_then drule>>
+  strip_tac>>
+  fs[satisfies_union]>>
+  qabbrev_tac`w' = flip_literal l w`>>
+  qexists_tac`w'` >> rw[satisfies_INSERT]>>
+  `l ≠ 0` by metis_tac[]
+  >- (
+    `satisfies_literal w' l` by
+      (simp[Abbr`w'`]>>
+      metis_tac[flip_literal_flips,satisfies_clause_def])>>
+    metis_tac[satisfies_clause_def])
+  >>
+    `fml = { D | D ∈ fml ∧ ¬MEM (-l) D} ∪ { D | D ∈ fml ∧ MEM (-l) D}` by
+      (simp[EXTENSION]>>
+      metis_tac[])>>
+    pop_assum SUBST1_TAC>>
+    rw[satisfies_union]
+    >- (
+      fs[satisfies_def]>>rw[]>>
+      fs[Abbr`w'`]>>
+      simp[Once flip_literal_eq_neg]>>
+      `-l ≠ 0` by fs[]>>
+      drule flip_literal_unaffected>>
+      disch_then match_mp_tac>> simp[]>>
+      metis_tac[satisfies_literal_exclusive,satisfies_clause_def])
+    >>
+      fs[satisfies_def]>>rw[]>>
+      `C ++ delete_literal (-l) C' ∈ Ds` by
+        (fs[Abbr`Ds`]>>
+        qexists_tac`C'`>>fs[])>>
+      first_x_assum drule>> disch_then kall_tac>>
+      first_x_assum drule>>
+      simp[satisfies_clause_append]>>
+      strip_tac>>
+      `satisfies_clause w' (delete_literal (-l) C')` by
+        (simp[Abbr`w'`]>>
+        simp[Once flip_literal_eq_neg]>>
+        `-l ≠ 0` by fs[]>>
+        drule flip_literal_unaffected>>
+        disch_then match_mp_tac>>
+        fs[delete_literal_def,MEM_FILTER]>>
+        metis_tac[satisfies_literal_exclusive,satisfies_clause_def])>>
+      pop_assum mp_tac>>
+      match_mp_tac satisfies_clause_SUBSET>>
+      fs[delete_literal_def,MEM_FILTER]
+QED
+
+(* More implementationy stuff *)
+
 val values_def = Define`
   values s = {v | ∃n. lookup n s = SOME v}`
+
+val wf_clause_def = Define`
+  wf_clause (C:clause) ⇔ ¬MEM 0 C`
 
 val wf_fml_def = Define`
   wf_fml fml ⇔ ∀C. C ∈ values fml ⇒ wf_clause C`
@@ -263,17 +406,117 @@ Proof
   metis_tac[unsatisfiable_def]
 QED
 
-Theorem UNION_INSERT_EQ:
-  A ∪ (B INSERT C) = B INSERT (A ∪ C)
+Theorem values_delete:
+  values (delete h v) ⊆ values v
 Proof
-  fs[EXTENSION]>>metis_tac[]
+  simp[values_def,lookup_delete,SUBSET_DEF]>>
+  metis_tac[]
 QED
+
+Theorem values_insert:
+  C ∈ values (insert n l fml) ⇒ C ∈ values fml ∨ C = l
+Proof
+  fs[values_def,lookup_insert]>>
+  rw[]>>
+  every_case_tac>>fs[]>>
+  metis_tac[]
+QED
+
+Theorem values_insert2:
+  values (insert n l fml) ⊆ l INSERT values fml
+Proof
+  rw[SUBSET_DEF]>>
+  metis_tac[values_insert]
+QED
+
+(*** Implementation ***)
+
+val _ = Datatype`
+  lratstep =
+    Delete (num list) (* Clauses to delete *)
+  | RAT num clause (num list) ((num list) spt)`
+    (* RAT step:
+      AT n C i0 (ik id ~> ik)
+      n is the new id of the new clause C
+      i0 is a list of clause IDs for the AT part
+      ik is a sptree mapping clause IDs to their hints
+    *)
+
+val _ = type_abbrev("lrat" , ``:lratstep list``);
+
+val delete_clauses_def = Define`
+  delete_clauses cl fml =
+    FOLDR delete fml cl`
+
+(*
+  Checking for asymmetric tautology via unit propagation using the given hints
+  NONE == Error
+  SOME (INL ()) == C is an AT
+  SOME (INR C) == hints were insufficient, but C is now extended with units
+*)
+val is_AT_def = Define`
+  (is_AT fml [] (C:clause) = SOME (INR C)) ∧
+  (is_AT fml (i::is) C =
+  case lookup i fml of
+    NONE => NONE
+  | SOME Ci =>
+  let D = FILTER (λx. ¬ MEM x C) Ci in
+  case D of
+    [] => SOME (INL ())
+  | [d] => is_AT fml is (-d::C)
+  | _ => NONE)`
+
+(*
+  Resolution Asymmetric Tautology
+*)
+val is_RAT_aux_def = Define`
+  (is_RAT_aux fml p C ik [] = T) ∧
+  (is_RAT_aux fml p C ik ((i,Ci)::iCs) =
+    if MEM (-p) Ci then
+      case lookup i ik of
+        NONE => F
+      | SOME is =>
+        if is_AT fml is (C ++ delete_literal (-p) Ci) = SOME (INL ()) then
+          is_RAT_aux fml p C ik iCs
+        else
+          F
+      (* Step 5.2 ????*)
+    else
+      is_RAT_aux fml p C ik iCs)`
+
+val is_RAT_def = Define`
+  is_RAT fml (C:clause) i0 ik =
+  (* First, do the asymmetric tautology check *)
+  case is_AT fml i0 C of
+    NONE => F
+  | SOME (INL ()) => T
+  | SOME (INR D) =>
+  (* First, do the asymmetric tautology check *)
+  case C of
+    [] => F
+  | (p::C) =>
+  let iCs = toAList fml in
+    is_RAT_aux fml p D ik iCs`
+
+(* Run the LRAT checker on fml, returning an option *)
+val check_lrat_def = Define`
+  (check_lrat [] fml = SOME fml) ∧
+  (check_lrat (step::steps) fml =
+    case step of
+      Delete cl =>
+      check_lrat steps (delete_clauses cl fml)
+    | RAT n C i0 ik =>
+      if wf_clause C then
+      if is_RAT fml C i0 ik then
+        check_lrat steps (insert n C fml)
+      else NONE
+      else NONE)`
 
 (* Implementation *)
 Theorem is_AT_imp_asymmetric_tautology:
   ∀is fml C.
-  wf_fml fml ∧ wf_clause C ⇒
-  is_AT fml is C ⇒
+  wf_fml fml ∧ wf_clause C ∧
+  is_AT fml is C = SOME (INL ()) ⇒
   asymmetric_tautology (values fml) C
 Proof
   Induct>>fs[is_AT_def]>>
@@ -322,14 +565,112 @@ Proof
     fs[UNION_INSERT_EQ]
 QED
 
-(* Deletion preserves sat: if C is satisfiable, then deleting clauses from C keeps satisfiability *)
-Theorem values_delete:
-  values (delete h v) ⊆ values v
+Theorem is_AT_imp_sat_preserving:
+  ∀is fml C D.
+  wf_fml fml ∧ wf_clause C ∧
+  is_AT fml is C = SOME (INR D) ⇒
+  ∃E.
+    D = E ++ C ∧ wf_clause D ∧
+    ∀w.
+    satisfies w (D INSERT values fml) ⇒
+    satisfies w (C INSERT values fml)
 Proof
-  simp[values_def,lookup_delete,SUBSET_DEF]>>
-  metis_tac[]
+  Induct>>fs[is_AT_def] >>
+  rw[]>>
+  every_case_tac>>fs[]>>
+  first_x_assum drule>>
+  `wf_clause (-h'::C)` by
+    (fs[wf_clause_def,wf_fml_def]>>
+    fs[values_def,PULL_EXISTS]>>
+    first_x_assum drule>>
+    `MEM h' (FILTER (λx. ¬MEM x C) x )` by fs[]>>
+    rw[]>>`h' ≠ 0` by metis_tac[MEM_FILTER]>>
+    intLib.ARITH_TAC)>>
+  disch_then drule>>
+  disch_then drule>>rw[]>>
+  qexists_tac`E++[-h']`>>fs[]>>
+  rw[]>>
+  first_x_assum drule>>
+  simp[satisfies_INSERT]>>
+  Cases_on`satisfies_clause w C`>>simp[]>>
+  Cases_on`satisfies w (values fml)`>> fs[] >>
+  `satisfies_clause w x` by
+    (fs[satisfies_def,values_def]>>metis_tac[])>>
+  `satisfies_literal w h'` by
+    (fs[satisfies_clause_def]>>
+    `¬MEM l C` by metis_tac[]>>
+    `MEM l (FILTER (λx. ¬MEM x C) x)` by
+      fs[MEM_FILTER]>>
+    rfs[]>>
+    metis_tac[])>>
+  PURE_REWRITE_TAC [Once CONS_APPEND]>>
+  simp[satisfies_clause_append,satisfies_clause_def]>>
+  `h' ≠ 0` by
+    (fs[wf_clause_def]>>
+    intLib.ARITH_TAC)>>
+  metis_tac[satisfies_literal_exclusive]
 QED
 
+Theorem is_RAT_aux_imp:
+  ∀iCs fml p C ik.
+  is_RAT_aux fml p C ik iCs ∧
+  wf_fml fml ∧
+  EVERY (λ(i,Ci). wf_clause Ci) iCs ∧
+  wf_clause C ⇒
+  ∀i Ci. MEM (i,Ci) iCs ∧ MEM (-p) Ci ⇒
+    asymmetric_tautology (values fml) (C ++ delete_literal (-p) Ci)
+Proof
+  Induct>>Cases>>fs[is_RAT_aux_def]>>
+  ntac 5 strip_tac >>
+  rw[]
+  >-
+    (last_x_assum kall_tac>> fs[]>>
+    every_case_tac>>fs[]>>
+    match_mp_tac is_AT_imp_asymmetric_tautology>> fs[]>>
+    qexists_tac`x`>>fs[wf_clause_def]>>
+    fs[delete_literal_def,MEM_FILTER])
+  >>
+    fs[PULL_FORALL,AND_IMP_INTRO]>>
+    first_x_assum match_mp_tac>>fs[]>>
+    every_case_tac>>fs[]>>metis_tac[]
+QED
+
+Theorem is_RAT_imp_resolution_asymmetric_tautology:
+  ∀fml C i0 ik.
+  wf_fml fml ∧ wf_clause C ∧
+  is_RAT fml C i0 ik ⇒
+  satisfiable (values fml) ⇒ satisfiable (C INSERT values fml)
+Proof
+  rw[is_RAT_def]>>
+  ntac 2 (pop_assum mp_tac)>> ntac 2 TOP_CASE_TAC>>fs[]
+  >-
+    (drule is_AT_imp_asymmetric_tautology>>
+    rpt (disch_then drule)>>
+    metis_tac[asymmetric_tautology_satisfiable]) >>
+  TOP_CASE_TAC>>fs[]>>
+  strip_tac>>
+  drule is_AT_imp_sat_preserving>>
+  disch_then drule>>
+  disch_then drule>>rw[]>>
+
+  qmatch_asmsub_abbrev_tac`wf_clause y`>>
+  drule is_RAT_aux_imp>> simp[]>>
+  `EVERY (λ(i,Ci). wf_clause Ci) (toAList fml)` by
+    (fs[EVERY_MEM,MEM_toAList,FORALL_PROD,wf_fml_def,values_def]>>
+    metis_tac[])>>
+  simp[MEM_toAList]>>
+  strip_tac>>
+  `resolution_asymmetric_tautology (values fml) y` by
+    (simp[resolution_asymmetric_tautology_def]>>
+    fs[wf_clause_def]>>
+    `MEM h y` by fs[Abbr`y`]>>
+    fs[values_def,PULL_EXISTS]>>
+    metis_tac[])>>
+  drule resolution_asymmetric_tautology_satisfiable>>
+  metis_tac[satisfiable_def]
+QED
+
+(* Deletion preserves sat: if C is satisfiable, then deleting clauses from C keeps satisfiability *)
 Theorem delete_preserves_satisfiable:
    satisfiable (values C) ⇒ satisfiable (values (delete n C))
 Proof
@@ -360,22 +701,6 @@ Proof
   fs[]
 QED
 
-Theorem values_insert:
-  C ∈ values (insert n l fml) ⇒ C ∈ values fml ∨ C = l
-Proof
-  fs[values_def,lookup_insert]>>
-  rw[]>>
-  every_case_tac>>fs[]>>
-  metis_tac[]
-QED
-
-Theorem values_insert2:
-  values (insert n l fml) ⊆ l INSERT values fml
-Proof
-  rw[SUBSET_DEF]>>
-  metis_tac[values_insert]
-QED
-
 Theorem wf_fml_insert:
   wf_fml fml ∧ wf_clause l ⇒
   wf_fml (insert n l fml)
@@ -398,20 +723,43 @@ Proof
     simp[]>>
     metis_tac[delete_clauses_sound,wf_fml_delete_clauses])
   >>
-    rw[]>>
-    drule wf_fml_insert>> disch_then drule>>
-    disch_then(qspec_then`n`assume_tac)>>
-    first_x_assum drule>>
-    disch_then drule>>
-    disch_then match_mp_tac>>
-    last_x_assum assume_tac>>
-    drule is_AT_imp_asymmetric_tautology>>
-    disch_then drule>>
-    disch_then drule>>
-    strip_tac>>drule (GEN_ALL asymmetric_tautology_satisfiable)>>
-    disch_then drule>>
-    match_mp_tac satisfiable_SUBSET>>
-    metis_tac[values_insert2]
+  rw[]>>
+  every_case_tac>>fs[]>>
+  drule wf_fml_insert>> disch_then drule>>
+  disch_then(qspec_then`n`assume_tac)>>
+  first_x_assum drule>>
+  disch_then drule>>
+  disch_then match_mp_tac>>
+  last_x_assum assume_tac>>
+  drule is_RAT_imp_resolution_asymmetric_tautology>>
+  disch_then drule>>
+  disch_then drule>>
+  disch_then drule>>
+  match_mp_tac satisfiable_SUBSET>>
+  metis_tac[values_insert2]
 QED
+
+(* Try on an example *)
+val fml = rconc (EVAL ``insert 1 [ 1;  2; -3] (
+  insert 2 [-1; -2;  3] (
+  insert 3 [ 2;  3; -4] (
+  insert 4 [-2; -3;  4] (
+  insert 5 [-1; -3; -4] (
+  insert 6 [ 1;  3;  4] (
+  insert 7 [-1;  2;  4] (
+  insert 8 [ (1:int); -2; -4] LN)))))))``)
+
+val lrat =
+``[
+  Delete [];
+  RAT 9 [-1] [] (insert 1 [5;7] (insert 6 [2;7] (insert 8 [5;2] LN)));
+  Delete [7;5;2] ;
+  RAT 10 [2] [9;1;6;3] LN;
+  Delete [1;3;0] ;
+  RAT 12 [] [9;10;8;4;6] LN
+]``;
+
+  (* result contains the empty clause *)
+val res = EVAL``toAList (THE (check_lrat ^(lrat) ^(fml)))``
 
 val _ = export_theory ();
